\Titelbanner{4}{Umgang mit Polynomen h√∂heren Grades\\
                Das Summenzeichen}

\textbf{Aufgabe 1: } \emph{Nullstellensuche}
\begin{enumerate}[label=(\alph*)]
\item $x^3-(a+b+c)x^2+(ab+ac+bc)x-abc$
\item $x^3+2x^4+4x^2+2+x=(x^2+1)(2x^2+x+2)$, keine (reellen) Nullstellen
\item $x_1=0$, \ \ $x_{2/3}=\pm\sqrt{2}$, \ \ $x_{4/5}=\pm 1$
\item $x_0\approx\frac{\pi}{2}$
\end{enumerate}
\vspace{0.7cm}
%
\textbf{Aufgabe 2: } \emph{Polynomdivision}
\begin{enumerate}[label=(\alph*)]
\item $(21a^3-34a^2b+25b^3):(7a+5b)=3a^2-7ab+5b^2$
\item $(9x^3-7xy^2+2y^3):(3x-2y)=3x^2+2xy-y^2$
\item $(25x^4+a^2x^2+25a^4):(5x^2+7ax+5a^2)=5x^2-7ax+5a^2$
\item $n=5$ oder $n=-3$, da $(x^2+2x-15)=(x+5)(x-3)$
\end{enumerate}
\vspace{0.7cm}
%
\textbf{Aufgabe 3: } \emph{Kubische Gleichungen}
\begin{enumerate}[label=(\alph*)]
\item $m=12$, $x_2=\frac{2}{3}$, $x_3=-\frac{3}{2}$
\item $m=-5$, $n=30$, $x_3=-\frac{5}{2}$
\end{enumerate}
\vspace{0.7cm}

%
\textbf{Aufgabe 4: } \emph{Nullstellenraten}
\begin{enumerate}[label=(\alph*)]
\item $x_0=1$ oder $x_0=2\ \ \ \Rightarrow\ x^3-5x^2+8x-4=(x-1)(x^2-4x+4)=(x-1)(x-2)^2$
\item $x_0=-3\ \Rightarrow\ x^4-2x^3-13x^2+9x+9=(x+3)(x^3-5x^2+2x+3)$
\item $x_0=-2\ \Rightarrow\ x^4-3x^2+3x+2=(x+2)(x^3-2x^2+x+1)$
\item $x_0=1\ \Rightarrow\ x^5-x^4-3x^3+3x^2+x-1=(x-1)(x^4-3x^2+1)$
\end{enumerate}
\vspace{0.7cm}
%
\newpage
\textbf{Aufgabe 5: } \emph{Partialbruchzerlegung}
\begin{enumerate}[label=(\alph*)]
\item $\frac{x-5}{x^2-2x-3}=\frac{3}{2(x+1)}-\frac{1}{2(x-3)}$
\item $\frac{x^2+1}{x^2-1}=1-\frac{1}{x+1}+\frac{1}{x-1}$
\item $\frac{2x^2-3x+1}{x^3-5x^2+8x-4}=\frac{2}{x-2}+\frac{3}{(x-2)^2}$
\item $\frac{2x^4-4x^3-5x^2+(\sqrt{2}-7)x+\sqrt{2}+12}{x^2-2x-3}=2x^2+1+\frac{\sqrt{2}}{x-3}-\frac{5}{x+1}$
\end{enumerate}
\vspace{0.7cm}
%

\textbf{Aufgabe 6: } \emph{Summen}
\begin{enumerate}[label=(\alph*), labelindent=1em,labelsep=0.5cm]
    \item $\sum_{k=1}^n \frac{1}{2k}+ \sum_{l=0}^{n-1} \frac{1}{2l+1} =\sum_{k=0}^{2n} \frac{1}{k}$
    \item $\sum_{k=1}^n \frac{1}{k(k+1)} = \frac{n}{n+1}$
    \item $\sum_{k=0}^n x^k = \frac{1 - x^{n+1}}{1-x}$ 
\end{enumerate}


% \textbf{Aufgabe 6: } \emph{Polynome in Ungleichungen}
% \begin{enumerate}[label=(\alph*)]
% \item $(1+a+a^2)^2<3(1+a^2+a^4)\ \ \ \Leftrightarrow\ \ \ 0<a^4-a^3-a+1=(a^3-1)(a-1)$ \hfill $\Box$
% \item $x^4-x^2-6x+10=(x^2-1)^2+(x-3)^2>0$ \hfill $\Box$
% \end{enumerate}